Some changes in the interpreter and in the proofs.

coq/JsCorrectness.v
@@ -542,14 +542,14 @@ Ltac run_ifres_select H :=
 (* [run_hyp H] exploits the induction hypothesis
    on [runs_type_correct] to the hypothesis [H] *)
 
-Ltac run_hyp_expr_get_value_if_to_string H := fail.
+Ltac run_hyp_conversions H := fail.
 
 Ltac run_hyp_select_proj H :=
   match type of H with
   | runs_type_expr _ _ _ _ = _ => constr:(runs_type_correct_expr)
   | runs_type_stat _ _ _ _ = _ => constr:(runs_type_correct_stat)
   | runs_type_prog _ _ _ _ = _ => constr:(runs_type_correct_prog)
-  | _ => run_hyp_expr_get_value_if_to_string H
+  | _ => run_hyp_conversions H
   end.
 
 Ltac run_hyp_select_ind tt :=
@@ -1035,11 +1035,43 @@ Admitted. (* OLD
              apply~ red_spec_object_default_value_4.
 Qed. *)
 
-Lemma to_string_correct : forall runs,
-  runs_type_correct runs -> forall S S' R' C v,
-  to_string runs S C v = out_ter S' R' ->
-  red_expr S C (spec_to_string v) (out_ter S' R') /\
-    (res_is_normal R' -> exists s, R' = prim_string s).
+
+(** Conversions *)
+
+Definition run_expr_get_value_post K o o1 :=
+  (eqabort o1 o \/
+    exists S1, exists (v1 : value), o1 = out_ter S1 v1 /\
+      K S1 v1 = result_out o).
+
+Lemma run_expr_get_value_correct : forall runs,
+  runs_type_correct runs -> forall S C e K o,
+  run_expr_get_value runs S C e K = o -> exists o1,
+    red_expr S C (spec_expr_get_value e) o1 /\
+      run_expr_get_value_post K o o1.
+Admitted.
+
+Definition if_to_primitive_post K o o1 :=
+  (eqabort o1 o \/
+    exists S, exists (w : prim), o1 = out_ter S w /\
+      K S w = result_out o).
+
+Lemma if_to_primitive_correct : forall runs,
+  runs_type_correct runs -> forall S C v prefo K o,
+  if_primitive (to_primitive runs S C v prefo) K = o -> exists o1,
+    red_expr S C (spec_to_primitive v prefo) o1 /\
+      if_to_primitive_post K o o1.
+Admitted.
+
+Definition if_to_string_post K o o1 :=
+  (eqabort o1 o \/
+    exists S, exists (s : string), o1 = out_ter S s /\
+      K S s = result_out o).
+
+Lemma if_to_string_correct : forall runs,
+  runs_type_correct runs -> forall S C v K o,
+  if_string (to_string runs S C v) K = o -> exists o1,
+    red_expr S C (spec_to_string v) o1 /\
+      if_to_string_post K o o1.
 Admitted. (* OLD
   introv RC E. destruct v; simpls.
    inverts E. splits*. apply~ red_spec_to_string_prim.
@@ -1054,18 +1086,39 @@ Admitted. (* OLD
      splits*. apply~ red_spec_to_string_1.
 Qed. *)
 
+Ltac run_hyp_conversions H ::=
+  match type of H with
+  | run_expr_get_value _ _ _ _ _ = _ => constr:(run_expr_get_value_correct)
+  | if_string (to_string _ _ _ _) _ = _ => constr:(if_to_string_correct)
+  end.
 
-Definition run_expr_get_value_post K o o1 :=
-  (eqabort o1 o \/
-    exists S1, exists (v1 : value), o1 = out_ter S1 v1 /\
-      K S1 v1 = result_out o).
+Ltac run_post_extra ::=
+  let Er := fresh "Er" in
+  let Ab := fresh "Ab" in
+  match goal with
+  | H: run_expr_get_value_post _ _ _ |- _ =>
+    let O1 := fresh "O1" in
+    let S1 := fresh "S" in
+    let v1 := fresh "v" in
+    destruct H as [(Er&Ab)|(S1&v1&O1&H)];
+    [ try abort_expr | try subst_hyp O1 ]
+  | H: if_string_to_string_post _ _ _ |- _ =>
+    let O1 := fresh "O1" in
+    let S1 := fresh "S" in
+    let s := fresh "s" in
+    destruct H as [(Er&Ab)|(S1&s&O1&H)];
+    [ try abort_expr | try subst_hyp O1 ]
+  end.
 
-Lemma run_expr_get_value_correct : forall runs,
-  runs_type_correct runs -> forall S C e K o,
-  run_expr_get_value runs S C e K = o -> exists o1,
-    red_expr S C (spec_expr_get_value e) o1 /\
-      run_expr_get_value_post K o o1.
-Admitted.
+Tactic Notation "run'" constr(Red) :=
+  match goal with H: _ = result_out _ |- _ =>
+    let T := fresh in rename H into T;
+    let o1 := fresh "o1" in let R1 := fresh "R1" in
+    run_hyp T as (o1&R1&R); applys Red (rm R1);
+    let o := run_get_current_out tt in
+    try (run_check_current_out o; run_post; run_inv)
+  end.
+
 
 (* OLD
 Ltac unmonad_passing :=
@@ -1111,51 +1164,6 @@ Ltac unmonad_passing :=
   dealing_follows;
   other_follows.
 *)
-
-Definition if_string_to_string_post K o o1 :=
-  (eqabort o1 o \/
-    exists S, exists (s : string), o1 = out_ter S s /\
-      K S s = result_out o).
-
-Lemma if_to_string_correct : forall runs,
-  runs_type_correct runs -> forall S C v K o,
-  if_string (to_string runs S C v) K = o -> exists o1,
-    red_expr S C (spec_to_string v) o1 /\
-      if_string_to_string_post K o o1.
-Admitted.
-
-Ltac run_hyp_expr_get_value_if_to_string H ::=
-  match type of H with
-  | run_expr_get_value _ _ _ _ _ = _ => constr:(run_expr_get_value_correct)
-  | if_string (to_string _ _ _ _) _ = _ => constr:(if_to_string_correct)
-  end.
-
-Ltac run_post_extra ::=
-  let Er := fresh "Er" in
-  let Ab := fresh "Ab" in
-  match goal with
-  | H: run_expr_get_value_post _ _ _ |- _ =>
-    let O1 := fresh "O1" in
-    let S1 := fresh "S" in
-    let v1 := fresh "v" in
-    destruct H as [(Er&Ab)|(S1&v1&O1&H)];
-    [ try abort_expr | try subst_hyp O1 ]
-  | H: if_string_to_string_post _ _ _ |- _ =>
-    let O1 := fresh "O1" in
-    let S1 := fresh "S" in
-    let s := fresh "s" in
-    destruct H as [(Er&Ab)|(S1&s&O1&H)];
-    [ try abort_expr | try subst_hyp O1 ]
-  end.
-
-Tactic Notation "run'" constr(Red) :=
-  match goal with H: _ = result_out _ |- _ =>
-    let T := fresh in rename H into T;
-    let o1 := fresh "o1" in let R1 := fresh "R1" in
-    run_hyp T as (o1&R1&R); applys Red (rm R1);
-    let o := run_get_current_out tt in
-    try (run_check_current_out o; run_post; run_inv)
-  end.
 
 
 (**************************************************************)
